Is0/Is0.lean
@@ -1,0 +1,32 @@
+import Mathlib.Data.Nat.Prime
+import Mathlib.Data.Vector
+import Mathlib.Data.ZMod.Defs
+import Mathlib.Data.ZMod.Basic
+import Mathlib.Tactic.LibrarySearch
+
+import Is0.Basic
+import Is0.Programs
+
+namespace Risc0
+
+lemma step_of_sequence_of_assign_eq_state_change :
+  ∀ (state : State) (name : String) (op : Op) (program : Cirgen),
+  Cirgen.step state (.Sequence (.Assign name op) program) = Cirgen.step (state.update name (Op.eval state op)) program := by
+  intros state name op program
+  cases op <;> {
+    conv =>
+      lhs
+      unfold Cirgen.step
+      simp only [State.update, Map.update, beq_iff_eq]
+  }
+
+theorem is0OriginalProgram_constraints_are_what_we_expect :
+  ∀ x y z : Felt, (is0OriginalProgram x y z).1.constraints.foldr And _root_.True ↔ (x = 0 ∧ x * x⁻¹ - 1 = 0) := by
+  intros x y z
+  apply Iff.intro
+  intros h
+  unfold is0OriginalProgram at h
+  sorry
+  sorry
+
+end Risc0
