Is0/Programs.lean
@@ -1,0 +1,83 @@
+import Mathlib.Data.Nat.Prime
+import Mathlib.Data.Vector
+import Mathlib.Data.ZMod.Defs
+import Mathlib.Data.ZMod.Basic
+import Mathlib.Tactic.LibrarySearch
+
+import Is0.Basic
+
+namespace Risc0
+
+-- The MLIR program labeled `ORIGINAL` in the `nonzero-example` output.
+def is0OriginalProgram (x : Felt) (y : Felt) (z : Felt) : State × Option Prop :=
+  Cirgen.step { felts := Map.empty
+              , props := Map.empty
+              , buffers := Map.fromList [("in", [x]), ("out", [y, z])]
+              , constraints := []
+              }
+    (.Sequence
+      (.Sequence
+        (.Sequence
+          (.Sequence
+            (.Sequence
+              (.Sequence
+                (.Sequence
+                  (.Sequence
+                    (.Sequence
+                      (.Assign "1" (Op.Const 1))
+                      (.Assign "x" (Op.Get ⟨"in"⟩ 0 0)))
+                      (.Assign "isZeroBit" (Op.Isz ⟨"x"⟩)))
+                      (.Set ⟨"out"⟩ 0 ⟨"isZeroBit"⟩))
+                      (.Assign "invVal" (Op.Inv ⟨"x"⟩)))
+                      (.Set ⟨"out"⟩ 1 ⟨"invVal"⟩))
+                      (.Assign "out[0]" (Op.Get ⟨"out"⟩ 0 0)))
+                      (.If ⟨"out[0]"⟩
+                        (.Eqz ⟨"x"⟩)))
+                      (.Assign "1 - out[0]" (Op.Sub ⟨"1"⟩ ⟨"out[0]"⟩)))
+                      (.If ⟨"1 - out[0]"⟩
+                        (.Sequence
+                          (.Sequence
+                            (.Sequence
+                              (.Assign "out[1]" (Op.Get ⟨"out"⟩ 1 0))
+                              (.Assign "x * out[1]" (Op.Mul ⟨"x"⟩ ⟨"out[1]"⟩)))
+                              (.Assign "x * out[1] - 1" (Op.Sub ⟨"x * out[1]"⟩ ⟨"1"⟩)))
+                              (.Eqz ⟨"x * out[1] - 1"⟩))))
+
+-- The MLIR program labeled `CONSTAINTS` in the `nonzero-example` output.
+def is0ConstraintsProgram (x : Felt) (y : Felt) (z : Felt) : State × Option Prop :=
+  Cirgen.step { felts := Map.empty
+              , props := Map.empty
+              , buffers := Map.fromList [("in", [x]), ("out", [y, z])]
+              , constraints := []
+              }
+  (.Sequence
+    (.Sequence
+      (.Sequence
+        (.Sequence
+          (.Sequence
+            (.Sequence
+              (.Sequence
+                (.Sequence
+                  (.Sequence
+                    (.Sequence
+                      (.Sequence
+                        (.Sequence
+                          (.Assign "1" (Op.Const 1))
+                          (.Assign "true" Op.True))
+                          (.Assign "x" (Op.Get ⟨"in"⟩ 0 0)))
+                          (.Assign "isZeroBit" (Op.Get ⟨"out"⟩ 0 0)))
+                          (.Assign "x = 0" (Op.AndEqz ⟨"true"⟩ ⟨"x"⟩)))
+                          (.Assign "IF isZeroBit THEN (x = 0) ELSE true" (Op.AndCond ⟨"true"⟩ ⟨"isZeroBit"⟩ ⟨"x = 0"⟩)))
+                          (.Assign "1 - isZeroBit" (Op.Sub ⟨"1"⟩ ⟨"isZeroBit"⟩)))
+                          (.Assign "invVal" (Op.Get ⟨"out"⟩ 1 0)))
+                          (.Assign "x * invVal" (Op.Mul ⟨"x"⟩ ⟨"invVal"⟩)))
+                          (.Assign "x * invVal - 1" (Op.Sub ⟨"x * invVal"⟩ ⟨"1"⟩)))
+                          (.Assign "x * invVal - 1 = 0" (Op.AndEqz ⟨"true"⟩ ⟨"x * invVal - 1"⟩)))
+                          (.Assign "result"
+                            (Op.AndCond
+                              ⟨"IF isZeroBit THEN (x = 0) ELSE true"⟩
+                              ⟨"1 - isZeroBit"⟩
+                              ⟨"x * invVal - 1 = 0"⟩)))
+                          (.Return "result"))
+
+end Risc0
